theories/goodman/models/hol_zf/Bacon_PP_ZF_Goodman_M1_Fn59.thy
@@ -1,0 +1,278 @@
+theory Bacon_PP_ZF_Goodman_M1_Fn59
+  imports
+    Bacon_PP_ZF_Tree_CEV_Soundness
+    "Higher_Order_Metaphysics_PP_Frontier.Bacon_PP_Goodman_M1_Complete"
+begin
+
+section \<open>Goodman M1 and Bacon's footnote 59 in the exact tree semantics\<close>
+
+context pp_t_moving_internal_parameters
+begin
+
+lemma pp_t_M1_fn59_liar_denotation:
+  assumes p: "Elem p (pp_t_domain Prop)"
+  shows "pp_t_holds
+      (pp_t_eval (pp_t_moving_internal_constants Pure) \<rho>
+        pp_M1_fn59_liar \<acute> p) w
+    \<longleftrightarrow>
+    (\<forall>X. Elem X (pp_t_domain pp_unary_ty) \<longrightarrow>
+      (\<forall>q. Elem q (pp_t_domain Prop) \<longrightarrow>
+        (Pure pp_unary_ty w X
+          \<and> pp_t_eqv Prop w q (pp_t_moving_seed w)
+          \<and> pp_t_eqv Prop w p (X \<acute> q)
+          \<longrightarrow> \<not> pp_t_holds (X \<acute> p) w)))"
+proof -
+  have beta:
+      "pp_t_eval (pp_t_moving_internal_constants Pure) \<rho>
+          pp_M1_fn59_liar \<acute> p
+       =
+       pp_t_eval (pp_t_moving_internal_constants Pure)
+          (extend_env p \<rho>)
+          (Forall pp_unary_ty
+            (Forall Prop
+              (Imp
+                (Conj
+                  (pp_pure pp_unary_ty (Var 1))
+                  (Conj
+                    (pp_fun Prop (Var 0))
+                    (Eq Prop (Var 2)
+                      (App (Var 1) (Var 0)))))
+                (Neg (App (Var 1) (Var 2))))))"
+    unfolding pp_M1_fn59_liar_def
+    using p by (simp add: Lambda_app)
+  show ?thesis
+    unfolding beta pp_pure_def pp_fun_def
+    apply (simp only: pp_t_eval_Forall_holds
+      pp_t_eval_Imp_holds pp_t_eval_Conj_holds
+      pp_t_eval_Neg_holds pp_t_eval_Eq_holds)
+    by (simp del: pp_t_eqv.simps
+      add: pp_t_classifier_holds extend_env.simps
+        pp_t_three_extensions_index_two
+        pp_t_moving_fundamental_at.simps pp_unary_ty_def)
+qed
+
+lemma pp_t_M1_fn59_QSS_denotation:
+  "pp_t_holds
+      (pp_t_eval (pp_t_moving_internal_constants Pure) \<rho> pp_QSS) w
+    \<longleftrightarrow>
+    (\<forall>X. Elem X (pp_t_domain pp_unary_ty) \<longrightarrow>
+      (\<forall>Y. Elem Y (pp_t_domain pp_unary_ty) \<longrightarrow>
+        (\<forall>q. Elem q (pp_t_domain Prop) \<longrightarrow>
+          (Pure pp_unary_ty w X
+            \<and> Pure pp_unary_ty w Y
+            \<and> pp_t_eqv Prop w q (pp_t_moving_seed w)
+            \<longrightarrow>
+            (pp_t_eqv Prop w (X \<acute> q) (Y \<acute> q)
+              \<longrightarrow> pp_t_eqv pp_unary_ty w X Y)))))"
+  unfolding pp_QSS_def pp_pure_def pp_fun_def
+  apply (simp only: pp_t_eval_Forall_holds
+    pp_t_eval_Imp_holds pp_t_eval_Conj_holds
+    pp_t_eval_Eq_holds)
+  by (simp del: pp_t_eqv.simps
+    add: pp_t_classifier_holds extend_env.simps
+      pp_t_three_extensions_index_two
+      pp_t_moving_fundamental_at.simps pp_unary_ty_def)
+
+theorem pp_t_M1_fn59_diagonal_contradiction:
+  fixes \<rho> :: "nat \<Rightarrow> ZF"
+  defines "D \<equiv>
+    pp_t_eval (pp_t_moving_internal_constants Pure) \<rho>
+      pp_M1_fn59_liar"
+  assumes D_pure: "Pure pp_unary_ty w D"
+    and qss_holds:
+      "pp_t_holds
+        (pp_t_eval (pp_t_moving_internal_constants Pure) \<rho> pp_QSS) w"
+  shows False
+proof -
+  let ?r = "pp_t_moving_seed w"
+  let ?d = "D \<acute> ?r"
+  have D_dom: "Elem D (pp_t_domain pp_unary_ty)"
+    unfolding D_def
+    using MovingTreeConstants.pp_t_eval_type[
+      OF typed_pp_M1_fn59_liar pp_t_empty_env_typed]
+    by (simp add: pp_t_dom_def)
+  have r_dom: "Elem ?r (pp_t_domain Prop)"
+    by (rule pp_t_moving_seed_in_domain)
+  have d_dom: "Elem ?d (pp_t_domain Prop)"
+    using D_dom r_dom unfolding pp_unary_ty_def
+    by (rule pp_t_app_closed)
+  have d_dom_unfolded:
+      "Elem
+        (pp_t_eval (pp_t_moving_internal_constants Pure) \<rho>
+          pp_M1_fn59_liar \<acute> ?r)
+        (pp_t_domain Prop)"
+    using d_dom unfolding D_def .
+  have diagonal:
+      "pp_t_holds (D \<acute> ?d) w
+        \<longleftrightarrow>
+       (\<forall>X. Elem X (pp_t_domain pp_unary_ty) \<longrightarrow>
+         (\<forall>q. Elem q (pp_t_domain Prop) \<longrightarrow>
+           (Pure pp_unary_ty w X
+             \<and> pp_t_eqv Prop w q ?r
+             \<and> pp_t_eqv Prop w ?d (X \<acute> q)
+             \<longrightarrow> \<not> pp_t_holds (X \<acute> ?d) w)))"
+    unfolding D_def
+    by (rule pp_t_M1_fn59_liar_denotation[OF d_dom_unfolded])
+  have qss:
+      "\<forall>X. Elem X (pp_t_domain pp_unary_ty) \<longrightarrow>
+        (\<forall>Y. Elem Y (pp_t_domain pp_unary_ty) \<longrightarrow>
+          (\<forall>q. Elem q (pp_t_domain Prop) \<longrightarrow>
+            (Pure pp_unary_ty w X
+              \<and> Pure pp_unary_ty w Y
+              \<and> pp_t_eqv Prop w q ?r
+              \<longrightarrow>
+              (pp_t_eqv Prop w (X \<acute> q) (Y \<acute> q)
+                \<longrightarrow> pp_t_eqv pp_unary_ty w X Y))))"
+    using qss_holds pp_t_M1_fn59_QSS_denotation by blast
+  have not_true:
+      "pp_t_holds (D \<acute> ?d) w \<Longrightarrow>
+        \<not> pp_t_holds (D \<acute> ?d) w"
+  proof -
+    assume true_Dd: "pp_t_holds (D \<acute> ?d) w"
+    have rhs:
+        "\<forall>X. Elem X (pp_t_domain pp_unary_ty) \<longrightarrow>
+          (\<forall>q. Elem q (pp_t_domain Prop) \<longrightarrow>
+            (Pure pp_unary_ty w X
+              \<and> pp_t_eqv Prop w q ?r
+              \<and> pp_t_eqv Prop w ?d (X \<acute> q)
+              \<longrightarrow> \<not> pp_t_holds (X \<acute> ?d) w))"
+      using diagonal true_Dd by blast
+    have rr: "pp_t_eqv Prop w ?r ?r"
+      by (rule pp_t_eqv_reflexive[OF r_dom])
+    have dd: "pp_t_eqv Prop w ?d (D \<acute> ?r)"
+      by (rule pp_t_eqv_reflexive[OF d_dom])
+    show "\<not> pp_t_holds (D \<acute> ?d) w"
+      using rhs D_dom r_dom D_pure rr dd by blast
+  qed
+  have true_if_not:
+      "\<not> pp_t_holds (D \<acute> ?d) w \<Longrightarrow>
+        pp_t_holds (D \<acute> ?d) w"
+  proof -
+    assume false_Dd: "\<not> pp_t_holds (D \<acute> ?d) w"
+    have rhs:
+        "\<forall>X. Elem X (pp_t_domain pp_unary_ty) \<longrightarrow>
+          (\<forall>q. Elem q (pp_t_domain Prop) \<longrightarrow>
+            (Pure pp_unary_ty w X
+              \<and> pp_t_eqv Prop w q ?r
+              \<and> pp_t_eqv Prop w ?d (X \<acute> q)
+              \<longrightarrow> \<not> pp_t_holds (X \<acute> ?d) w))"
+    proof (intro allI impI)
+      fix X q
+      assume X_dom: "Elem X (pp_t_domain pp_unary_ty)"
+        and q_dom: "Elem q (pp_t_domain Prop)"
+        and antecedent:
+          "Pure pp_unary_ty w X
+            \<and> pp_t_eqv Prop w q ?r
+            \<and> pp_t_eqv Prop w ?d (X \<acute> q)"
+      then have X_pure: "Pure pp_unary_ty w X"
+        and qr: "pp_t_eqv Prop w q ?r"
+        and d_Xq: "pp_t_eqv Prop w ?d (X \<acute> q)"
+        by auto
+      have Xq_dom: "Elem (X \<acute> q) (pp_t_domain Prop)"
+        using X_dom q_dom unfolding pp_unary_ty_def
+        by (rule pp_t_app_closed)
+      have Xr_dom: "Elem (X \<acute> ?r) (pp_t_domain Prop)"
+        using X_dom r_dom unfolding pp_unary_ty_def
+        by (rule pp_t_app_closed)
+      have Xq_Xr: "pp_t_eqv Prop w (X \<acute> q) (X \<acute> ?r)"
+        using X_dom q_dom r_dom qr unfolding pp_unary_ty_def
+        by (rule pp_t_arrow_member_respects)
+      have d_Xr: "pp_t_eqv Prop w ?d (X \<acute> ?r)"
+        using d_dom Xq_dom Xr_dom d_Xq Xq_Xr
+        by (rule pp_t_eqv_transitive)
+      have rr: "pp_t_eqv Prop w ?r ?r"
+        by (rule pp_t_eqv_reflexive[OF r_dom])
+      have D_X: "pp_t_eqv pp_unary_ty w D X"
+        using qss D_dom X_dom r_dom D_pure X_pure rr d_Xr
+        by blast
+      have dd: "pp_t_eqv Prop w ?d ?d"
+        by (rule pp_t_eqv_reflexive[OF d_dom])
+      have Dd_Xd: "pp_t_eqv Prop w (D \<acute> ?d) (X \<acute> ?d)"
+        using D_X d_dom d_dom dd unfolding pp_unary_ty_def
+        by (rule pp_t_app_respects)
+      show "\<not> pp_t_holds (X \<acute> ?d) w"
+        using false_Dd pp_t_prop_eqv_at[OF Dd_Xd, of w]
+        by blast
+    qed
+    show "pp_t_holds (D \<acute> ?d) w"
+      using diagonal rhs by blast
+  qed
+  show False
+    using not_true true_if_not by blast
+qed
+
+theorem pp_t_M1_fn59_PP_failure:
+  assumes background_valid:
+      "MovingTreeConstants.TreeHenkin.gvalid_set
+        (pp_M1_fn59_axioms - {pp_target_PP})"
+    and qss_valid:
+      "MovingTreeConstants.TreeHenkin.gvalid [] pp_QSS"
+  shows "\<not> MovingTreeConstants.TreeHenkin.gvalid [] pp_target_PP"
+proof
+  assume PP_valid:
+    "MovingTreeConstants.TreeHenkin.gvalid [] pp_target_PP"
+  have PP_all:
+      "\<And>\<Gamma>. MovingTreeConstants.TreeHenkin.gvalid
+        \<Gamma> pp_target_PP"
+    using typed_pp_target_PP PP_valid
+    by (rule MovingTreeConstants.pp_t_closed_gvalid_all_contexts)
+  have axioms_valid:
+      "MovingTreeConstants.TreeHenkin.gvalid_set pp_M1_fn59_axioms"
+    unfolding MovingTreeConstants.TreeHenkin.gvalid_set_def
+  proof (intro allI impI)
+    fix \<Gamma> A
+    assume "A \<in> pp_M1_fn59_axioms"
+    then show
+      "MovingTreeConstants.TreeHenkin.gvalid \<Gamma> A"
+    proof (cases "A = pp_target_PP")
+      case True
+      then show ?thesis using PP_all by simp
+    next
+      case False
+      then have "A \<in> pp_M1_fn59_axioms - {pp_target_PP}"
+        using \<open>A \<in> pp_M1_fn59_axioms\<close> by blast
+      then show ?thesis
+        using background_valid
+        unfolding MovingTreeConstants.TreeHenkin.gvalid_set_def
+        by blast
+    qed
+  qed
+  have liar_pure_valid:
+      "MovingTreeConstants.TreeHenkin.gvalid []
+        (pp_pure pp_unary_ty pp_M1_fn59_liar)"
+    using MovingTreeConstants.pp_t_base_sound
+      MovingTreeConstants.pp_t_zeta_sound
+      axioms_valid pp_M1_fn59_liar_pure
+    by (rule MovingTreeConstants.TreeHenkin.CEV_axiom_soundness)
+  let ?rho = "pp_t_list_env []"
+  have pure_holds:
+      "pp_t_holds
+        (pp_t_eval (pp_t_moving_internal_constants Pure) ?rho
+          (pp_pure pp_unary_ty pp_M1_fn59_liar)) w"
+    using MovingTreeConstants.TreeHenkin.gvalidD[
+      OF liar_pure_valid, of "[]" w]
+    unfolding MovingTreeConstants.pp_t_den_def
+    by simp
+  have D_pure:
+      "Pure pp_unary_ty w
+        (pp_t_eval (pp_t_moving_internal_constants Pure) ?rho
+          pp_M1_fn59_liar)"
+    using pure_holds
+      pp_t_moving_eval_pure_holds[
+        OF typed_pp_M1_fn59_liar pp_t_empty_env_typed]
+    by blast
+  have qss_holds:
+      "pp_t_holds
+        (pp_t_eval (pp_t_moving_internal_constants Pure) ?rho pp_QSS) w"
+    using MovingTreeConstants.TreeHenkin.gvalidD[
+      OF qss_valid, of "[]" w]
+    unfolding MovingTreeConstants.pp_t_den_def
+    by simp
+  show False
+    using D_pure qss_holds
+    by (rule pp_t_M1_fn59_diagonal_contradiction)
+qed
+
+end
+
+end
